tests/lean/combinators1.lean
@@ -2,10 +2,10 @@ open tactic
 
 example (p q : Prop) : p → q → (p ∧ p) ∧ q :=
 by do
-  intros, constructor, focus [trace "first goal" >> trace_state >> constructor, trace "--- Second goal: " >> trace_state >> assumption],
+  intros, constructor, focus [trace "first goal" >> trace_state >> constructor >> skip, trace "--- Second goal: " >> trace_state >> assumption],
   trace "--- After", trace_state,
   solve [trace "should not work", assumption],
-  first [trace "should not work" >> failed, constructor, trace "should work" >> assumption]
+  first [trace "should not work" >> failed, constructor >> skip, trace "should work" >> assumption]
 
 example (p q : Prop) : p → q → p ∧ q :=
-by do intros, constructor; assumption
+by do intros, constructor >> skip; assumption
