tests/lean/run/handthen.lean
@@ -3,7 +3,7 @@ open tactic
 lemma ex1 (a b c : nat) : a + 0 = 0 + a ∧ b = b :=
 begin
   -- We use `(` to go to regular tactic mode.
-  (constructor; [skip, constructor]),
+  constructor; [skip, constructor],
   -- Remaining goal is
   -- |- a + 0 = 0 + a
   simp
